\documentclass[crop=false,class=book,oneside]{standalone}
%----------------------------Preamble-------------------------------%
\input{../../../preamble.tex}
%--------------------------Main Document----------------------------%
\begin{document}
    \ifx\ifmath\undefined
        \title{Calculus I}
        \author{Ryan Maguire}
        \date{\vspace{-5ex}}
        \maketitle
        \tableofcontents
        \chapter*{Calculus I}
        \addcontentsline{toc}{chapter}{Calculus I}
        \markboth{}{CALCULUS I}
        \setcounter{chapter}{1}
    \else
        \chapter{Calculus I}
    \fi
    \section{Exams}
        \subsection{CLEP Exam}
            \begin{problem}
                If $f(x)=-2x^{-3}$, then $f'(x)=$
                \begin{enumerate}[label=(\Alph*)]
                    \begin{multicols}{4}
                        \item Bob
                        \item Bill
                        \item Alice
                        \item George
                    \end{multicols}
                \end{enumerate}
            \end{problem}
            \clearpage
        \subsection{Exam I}
            \begin{problem}
            Compute the derivative of $y(x)=\frac{1}{2}(x^{4}+7)$
            \end{problem}
            \begin{proof}[Solution]
            $\frac{dy}{dx}=\frac{d}{dx}(\frac{1}{2}(x^{4}+7))=\frac{1}{2}\frac{d}{dx}(x^{4}+7)=\frac{1}{2}(4x^{3})=2x^{3}$
            \end{proof}
            \begin{problem}
            Compute the derivative of $y(x)=\frac{x^{2}+1}{5}$
            \end{problem}
            \begin{proof}[Solution]
            $\frac{dy}{dx}=\frac{d}{dx}(\frac{x^{2}+1}{5})=\frac{1}{5}\frac{d}{dx}(x^{2}+1)=\frac{1}{5}(2x)=\frac{2}{5}x$
            \end{proof}
            \begin{problem}
            Compute the derivative of $y(x)=-3x^{-8}+2\sqrt{x}$
            \end{problem}
            \begin{proof}[Solution]
            $\frac{dy}{dx}=\frac{d}{dx}(3x^{-8}+2\sqrt{x})=3\frac{d}{dx}(x^{-8})+2\frac{d}{dx}(x^{\frac{1}{2}})=-24x^{9}+x^{-\frac{1}{2}}$
            \end{proof}
            \begin{problem}
            Compute the derivative of $y(x)=\frac{x\sqrt{x}+1}{x}$
            \end{problem}
            \begin{proof}[Solution]
            $\frac{dy}{dx}=\frac{d}{dx}(\frac{x\sqrt{x}+1}{x})=\frac{d}{dx}(x^{\frac{1}{2}}+x^{-1})=\frac{d}{dx}(x^{\frac{1}{2}})+\frac{d}{dx}(x^{-1})=\frac{1}{2}x^{-\frac{1}{2}}-x^{-2}$
            \end{proof}
            \begin{problem}
            Compute the derivative of $y(x)=\frac{\sqrt{x}+\sqrt[3]{x}}{\sqrt[4]{x^{3}}}$
            \end{problem}
            \begin{proof}[Solution]
            $\frac{dy}{dx}=\frac{d}{dx}(\frac{\sqrt{x}+\sqrt[3]{x}}{\sqrt[4]{x^{3}}})=\frac{d}{dx}(x^{\frac{1}{2}-\frac{3}{4}}+x^{\frac{1}{3}-\frac{3}{4}})=\frac{d}{dx}(x^{-\frac{1}{4}})+\frac{d}{dx}(x^{-\frac{5}{12}})=-\frac{1}{4}x^{-\frac{5}{4}}-\frac{5}{12}x^{-\frac{17}{12}}$
            \end{proof}
            \begin{problem}
            Compute the derivative of $y(t)=\frac{t^{2}+1}{3t}$
            \end{problem}
            \begin{proof}[Solution]
            $\frac{dy}{dt}=\frac{d}{dt}(\frac{t^{2}+1}{3t})=\frac{1}{3}\frac{d}{dt}(t+t^{-1})=\frac{1}{3}(\frac{d}{dt}(t)+\frac{d}{dt}(t^{-1}))=\frac{1-t^{-2}}{3}$
            \end{proof}
            \begin{problem}
            What are the horizontal tangents of $g(t)=e^{t}-4t+5$?
            \end{problem}
            \begin{proof}[Solution]
            Horizontal tangents occur when $\frac{dg}{dt}=0$. Computing, we have: $\frac{dg}{dt}=\frac{d}{dt}(e^{t}-4t+5) = e^{t}-4$. So $\frac{dg}{dt}=0\Rightarrow e^{t}-4=0\Rightarrow e^{t}=4\Rightarrow t=\ln(4)=2\ln(2)$. There is a horizontal tangent at $t=2\ln(2)$.
            \end{proof}
            \begin{problem}
            Compute $\frac{d^{2}y}{dx^{2}}$ of $x\sin(x)$. Simplify.
            \end{problem}
            \begin{proof}[Solution]
            $\frac{d^{2}y}{dx^{2}}=\frac{d}{dx}(\frac{dy}{dx})$. Computing the first derivative, we have:
            \begin{equation*}
                \frac{dy}{dx}=\frac{d}{dx}(x\sin(x))=x\frac{d}{dx}(\sin(x))+\sin(x)\frac{d(x)}{dx}=x\cos(x)+\sin(x)    
            \end{equation*}
            Computing the second derivative, we have:
            \begin{equation*}
            \frac{d^{2}y}{dx^{2}}=\frac{d}{dx}(\frac{dy}{dx})=\frac{d}{dx}(x\cos(x)+\sin(x))=\frac{d}{dx}(x\cos(x))+\frac{d}{dx}(\sin(x)) =-x\sin(x)+\cos(x)+\cos(x)   
            \end{equation*}
            Simplifying, we have $\frac{d^{2}y}{dx^{2}} = 2\cos(x)-x\sin(x)$
            \end{proof}
            \begin{problem}
            Compute the derivative of $f(t)=\frac{2t-1}{t+3}$
            \end{problem}
            \begin{proof}[Solution]
            $\frac{df}{dt}=\frac{d}{dt}(\frac{2t-1}{t+3})=\frac{(t+3)\frac{d}{dt}(2t-1)-(2t-1)\frac{d}{dt}(t+3)}{(t+3)^{2}}=\frac{2(t+3)-(2t-1)}{(t+3)^{2})}=\frac{7}{(t+3)^{2}}$
            \end{proof}
            \begin{problem}
            Compute the derivative of $g(x)=\frac{x^{2}-1}{x^{2}+1}$
            \end{problem}
            \begin{proof}[Solution]
            $\frac{dg}{dx}=\frac{d}{dx}(\frac{x^{2}-1}{x^{2}+1})=\frac{(x^{2}+1)\frac{d}{dx}(x^{2}-1)-(x^{2}-1)\frac{d}{dx}(x^{2}+1)}{(x^{2}+1)^{2}}=\frac{2x((x^{2}+1)-(x^{2}-1))}{(x^{2}+1)^{2}}=\frac{4x}{(x^{2}+1)^{2}}$
            \end{proof}
            \begin{problem}
            Compute the derivative of $h(x)=\frac{x}{x^{2}+1}$
            \end{problem}
            \begin{proof}[Solution]
            $\frac{dh}{dx}=\frac{d}{dx}(\frac{x}{x^{2}+1})=\frac{(x^{2}+1)\frac{d(x)}{dx}-x\frac{d}{dx}(x^{2}+1)}{(x^{2}+1)^{2}}=\frac{(x^{2}+1)-2x^{2}}{(x^{2}+1)^{2}}=\frac{1-x^{2}}{(x^{2}+1)^{2}}$
            \end{proof}
            \begin{problem}
            Compute the derative of $y(t)=\frac{3t^{2}-5}{2t+1}$
            \end{problem}
            \begin{proof}[Solution]
            $\frac{dy}{dt}=\frac{d}{dt}(\frac{3t^{2}-5}{2t+1})=\frac{(2t+1)\frac{d}{dt}(3t^{2}-5)-(3t^{2}-5)\frac{d}{dt}(2t+1)}{(2t+1)^{2}}=\frac{(2t+1)(6t)-(3t^{2}-5)(2)}{(2t+1)^{2}}=\frac{6t^{2}+6t+10}{2}$
            \end{proof}
            \begin{problem}
            Find the equation of the tangent line to the graph of $f(x)=x-2\tan(x)$ at $x=\frac{\pi}{4}$.
            \end{problem}
            \begin{proof}[Solution]
            The equation of the tangent is $y(x)=f'(x_{0})(x-x_{0})+f(x_{0})$. Computing the derivative, we have: $\frac{df}{dx}=\frac{d}{dx}(x-2\tan(x))=1-2\sec^{2}(x)$. So $f'(\frac{\pi}{4})=-3$. And $f(\frac{\pi}{4})=\frac{\pi}{4}-2\tan(\frac{\pi}{4})=\frac{\pi}{4}-2$. The tangent is $y(x)=-3(x-\frac{\pi}{4})+\frac{\pi}{4}-2$. Simplifying, we get $y(x)=-3x+\pi-2$
            \end{proof}
            \newpage
            \begin{problem}
            Use the limit definition to compute the derivative of $f(x)=\frac{1}{x}$.
            \end{problem}
            \begin{proof}[Solution]
            \begin{equation*}
                \frac{df}{dx}(x)=\underset{h\rightarrow 0}{\lim}\frac{f(x+h)-f(x)}{h}=\underset{h\rightarrow 0}{\lim}\frac{\frac{1}{x+h}-\frac{1}{x}}{h}=\underset{h\rightarrow 0}{\lim}\frac{\frac{x-(x+h)}{x(x+h)}}{h}=\underset{h\rightarrow 0}{\lim}-\frac{1}{x(x+h)}=-\frac{1}{x^{2}}
            \end{equation*}
            \end{proof}
            \begin{problem}
            Use the limit definition to compute the derivative of $f(x)=\frac{1}{x+1}$
            \end{problem}
            \begin{proof}[Solution]
            \begin{align*}
                \frac{df}{dx}(x)&=\underset{h\rightarrow 0}{\lim}\frac{f(x+h)-f(x)}{h}=\underset{h\rightarrow 0}{\lim}\frac{\frac{1}{x+h+1}-\frac{1}{x+1}}{h}=\underset{h\rightarrow 0}{\lim}\frac{\frac{x+1-(x+h+1)}{(x+1)(x+h+1)}}{h}\\
                &=\underset{h\rightarrow 0}{\lim}-\frac{1}{(x+h+1)(x+1)}=-\frac{1}{(x+1)^{2}}
            \end{align*}
            \end{proof}
            \begin{problem}
            Use the limit definition to compute the derivative of $f(x)=\frac{1}{\sqrt{x}}$
            \end{problem}
            \begin{proof}[Solution]
            \begin{align*}
                \frac{df}{dx}(x)&=\underset{h\rightarrow 0}{\lim}\frac{f(x+h)-f(x)}{h}=\underset{h\rightarrow 0}{\lim}\frac{\frac{1}{\sqrt{x+h}}-\frac{1}{\sqrt{x}}}{h}=\underset{h\rightarrow 0}{\lim}\frac{\frac{\sqrt{x}-\sqrt{x+h}}{\sqrt{x+h}\sqrt{x}}}{h}=\underset{h\rightarrow 0}{\lim}\frac{x-(x+h)}{h\sqrt{x+h}\sqrt{x}(\sqrt{x+h}+\sqrt{x})}\\
                &=\underset{h\rightarrow 0}{\lim}-\frac{1}{\sqrt{x+h}\sqrt{x}(\sqrt{x+h}+\sqrt{x})}=-\frac{1}{x\sqrt{x}}
            \end{align*}
            \end{proof}
            \begin{problem}
            use the limit definition to compute the derivative of $f(x)=\frac{1}{x^{2}}$
            \end{problem}
            \begin{proof}[Solution]
            \begin{equation*}
                \frac{df}{dx}(x)=\underset{h\rightarrow 0}{\lim}\frac{f(x+h)-f(x)}{h}=\underset{h\rightarrow 0}{\lim}\frac{\frac{1}{(x+h)^{2}}-\frac{1}{x^{2}}}{h}=\underset{h\rightarrow 0}{\lim}\frac{\frac{x^{2}-(x+h)^{2}}{x^{2}(x+h)^{2}}}{h}=\underset{h\rightarrow 0}{\lim}-\frac{2x+h^{2}}{x^{2}(x+h)^{2}}=-\frac{2}{x^{3}}
            \end{equation*}
            \end{proof}
            \begin{problem}
            Use the limit definition to compute the derivative of $f(x)=\sqrt{x+1}$
            \end{problem}
            \begin{proof}[Solution]
            \begin{align*}
                \frac{df}{dx}(x)&=\underset{h\rightarrow 0}{\lim}\frac{f(x+h)-f(x)}{h}=\underset{h\rightarrow 0}{\lim}\frac{\sqrt{x+h+1}-\sqrt{x+1}}{h}=\underset{h\rightarrow 0}{\lim}\frac{(x+h+1)-(x+1)}{h(\sqrt{x+h+1}+\sqrt{x+1})}\\
                &=\underset{h\rightarrow 0}{\lim}\frac{1}{\sqrt{x+h+1}+\sqrt{x+1}}=\frac{1}{2\sqrt{x+1}}
            \end{align*}
            \end{proof}
            \begin{problem}
            Find the horizontal and vertical asymptotes of $f(x)=\frac{2x^{3}-3}{x^{4}-16}$
            \end{problem}
            \begin{proof}[Solution]
            Horizontal asymptotes occur when the limit $\underset{x\rightarrow\pm}{\lim}f(x)$ exists. For both limits $f(x)\rightarrow 0$, from L'H\^{o}pital's rule. Vertical asymptotes occur when the denominator approaches 0. This occurs when $x^{4}=16$. The real solutions to this are $x=2$ and $x=-2$. From this we get:
            \begin{align*}
                \underset{x\rightarrow 2^{+}}{\lim}f(x)&=+\infty&\underset{x\rightarrow 2^{-}}{\lim}f(x)&=-\infty&\underset{x\rightarrow -2^{+}}{\lim}f(x)&=-\infty&\underset{x\rightarrow -2^{-}}{\lim}f(x)&=+\infty
            \end{align*}
            \end{proof}
            \begin{problem}
            Evaluate $\underset{x\rightarrow\infty}{\lim}\frac{3x^{4}+5}{2x^{4}}$
            \end{problem}
            \begin{proof}[Solution]
            From L'H\^{o}pital's Rule: $\underset{x\rightarrow\infty}{\lim}\frac{3x^{4}+5}{2x^{4}}=\underset{x\rightarrow\infty}{\lim}\frac{12x^{3}}{8x^{3}}=\underset{x\rightarrow \infty}{\lim}\frac{3}{2}=\frac{3}{2}$
            \end{proof}
        \subsection{Exam II}
            \begin{problem}
            Compute the derivative of $f(x)=e^{\sec(x)}$
            \end{problem}
            \begin{proof}[Solution]
            From the chain rule: $\frac{df}{dx}(x)=\frac{d}{dx}(e^{\sec(x)})=e^{\sec(x)}\frac{d}{dx}(\sec(x))=e^{\sec(x)}\sec(x)\tan(x)$
            \end{proof}
            \begin{problem}
            Compute the derivative of $g(x)=\ln(\sin^{2}(x))$
            \end{problem}
            \begin{proof}[Solution]
            Chain rule: $\frac{dg}{dx}(x)=\frac{d}{dx}(\ln(\sin^{2}(x)))=\frac{1}{\sin^{2}(x)}\frac{d}{dx}(\sin^{2}(x))=\frac{2\sin(x)\cos(x)}{\sin^{2}(x)}=2\cot(x)$
            \end{proof}
            \begin{problem}
            Compute the derivative of $s(t)=\sin(\sqrt[5]{t})$
            \end{problem}
            \begin{proof}[Solution]
            Chain rule: $\frac{ds}{dt}(t)=\frac{d}{dt}(\sin(\sqrt[5]{t}))=\cos(\sqrt[5]{t})\frac{d}{dt}(\sqrt[5]{t})=\frac{\cos(\sqrt[5]{t})}{5\sqrt[5]{t^{4}}}$
            \end{proof}
            \begin{problem}
            Compute the derivative of $f(x)=\ln(\cos^{-1}(x))$
            \end{problem}
            \begin{proof}[Solution]
            Chain rule: $\frac{df}{dx}(x)=\frac{d}{dx}(\ln(\cos^{-1}(x)))=\frac{1}{\cos^{-1}(x)}\frac{d}{dx}(\cos^{-1}(x))=-\frac{1}{\cos^{-1}(x)\sqrt{1-x^{2}}}$
            \end{proof}
            \begin{problem}
            Compute the derivative of $y(x)=(x+2)^{x+2}$
            \end{problem}
            \begin{proof}[Solution]
            Let $f(x)=\ln(y(x))$. Then $f(x)=\ln((x+2)^{x+2})=(x+2)\ln(x+2)$. Then:
            \begin{equation*}
                \frac{df}{dx}(x)=(x+2)\frac{d}{dx}(\ln(x+2))+\ln(x+2)\frac{d}{dx}(x+2)=1+\ln(x+2)
            \end{equation*}
            But $\frac{df}{dx}(x)=\frac{d}{dx}(\ln(y(x)))=\frac{1}{y(x)}\frac{dy}{dx}(x)$, so $\frac{dy}{dx}(x)=y(x)\frac{df}{dx}(x)$. Thus, $\frac{dy}{dx}(x)=(x+2)^{x+2}(1+\ln(x+2))$
            \end{proof}
            \begin{problem}
            Compute the derivative of $\sqrt{xy}=1$
            \end{problem}
            \begin{proof}[Solution]
            $\frac{d}{dx}(\sqrt{xy})=\frac{d}{dx}(1)=0$. And $\sqrt{xy}=1\Rightarrow xy=1\Rightarrow y=\frac{1}{x}$. So:
            \begin{equation*}
                \frac{1}{\sqrt{xy}}\frac{d}{dx}(xy)=0\Rightarrow \frac{y}{\sqrt{xy}}+\frac{x}{\sqrt{xy}}\frac{dy}{dx}=0\Rightarrow y+x\frac{dy}{dx}=0\Rightarrow\frac{dy}{dx}=-\frac{y}{x}=\frac{dy}{dx}=-\frac{1}{x^{2}}
            \end{equation*}
            \end{proof}
            \begin{problem}
            Compute the derivative of $y(x)=x^{2}\cos^{2}(2x^{2})$
            \end{problem}
            \begin{proof}[Solution]
            $\frac{d}{dx}(x^{2}\cos^{2}(2x^{2}))=\cos^{2}(2x^{2})\frac{d}{dx}(x^{2})+x^{2}\frac{d}{dx}(\cos^{2}(2x^{2}))=2x\cos^{2}(2x^{2})+8x^{3}\sin^{2}(2x^{2})$
            \end{proof}
            \begin{problem}
            Compute the derivative of $y(t)=t\tan^{-1}(t)-\frac{1}{2}\ln(t)$
            \end{problem}
            \begin{proof}[Solution]
            $\frac{dy}{dt}(t)=\frac{d}{dt}(t\tan^{-1}(t))-\frac{1}{2}\frac{d}{dt}(\ln(t))=\tan^{-1}(t)+t\frac{d}{dt}(\tan^{-1}(t))-\frac{1}{2t}=\tan^{-1}(t)+\frac{t}{1+t^{2}}-\frac{1}{2t}$
            \end{proof}
            \begin{problem}
            Compute the derivative of $f(x)=xe^{\sqrt[3]{x}}$
            \end{problem}
            \begin{proof}[Solution]
            $\frac{df}{dx}(x)=\frac{d}{dx}(xe^{\sqrt[3]{x}})=e^{\sqrt[3]{x}}+xe^{\sqrt[3]{x}}\frac{d}{dx}(\sqrt[3]{x})=e^{\sqrt[3]{x}}+\frac{1}{3}\sqrt[3]{x}e^{\sqrt[3]{x}}$
            \end{proof}
            \begin{problem}
            Compute the derivative of $g(x)=\ln(\csc(x^{2}))$
            \end{problem}
            \begin{proof}[Solution]
            $\frac{d}{dx}(\ln(\csc(x^{2})))=\frac{1}{\csc(x^{2})}\frac{d}{dx}(\csc(x^{2}))=-\sin(x^{2})\cot(x^{2})\csc(x^{2})\frac{d}{dx}(x^{2})=-2x\cot(x^{2})$
            \end{proof}
            \begin{problem}
            Compute the derivative of $s(t)=\sin(\tan(t))$
            \end{problem}
            \begin{proof}[Solution]
            $\frac{ds}{dt}(t)=\frac{d}{dt}(\sin(\tan(t)))=\cos(\tan(t))\frac{d}{dt}(\tan(t))=\cos(\tan(t))\sec^{2}(t)$
            \end{proof}
            \begin{problem}
            Compute the derivative of $f(x)=e^{\tan(x)}$
            \end{problem}
            \begin{proof}[Solution]
            $\frac{df}{dx}(x)=\frac{d}{dx}(e^{\tan(x)})=e^{\tan(x)}\frac{d}{dx}(\tan(x))=e^{\tan(x)}\sec^{2}(x)$
            \end{proof}
            \begin{problem}
            Compute the derivative of $g(x)=\ln(\sec(x))$
            \end{problem}
            \begin{proof}[Solution]
            $\frac{dg}{dx}(x)=\frac{d}{dx}(\ln(\sec(x)))=\frac{1}{\sec(x)}\frac{d}{dx}(\sec(x))=\tan(x)$
            \end{proof}
            \begin{problem}
            Compute the derivative of $s(t)=\cos(\sqrt{1+t^{2}})$
            \end{problem}
            \begin{proof}[Solution]
            $\frac{ds}{dt}(t)=\frac{d}{dt}(\cos(\sqrt{1+t^{2}}))=-\sin(\sqrt{1+t^{2}})\frac{d}{dt}(\sqrt{1+t^{2}})=-\frac{t}{\sqrt{1+t^{2}}}\sin(\sqrt{1+t^{2}})$
            \end{proof}
            \begin{problem}
            Compute the second derivative of $y(x)=\sin^{-1}(2x)$
            \end{problem}
            \begin{proof}[Solution]
            The second derivative is $\frac{d^{2}y}{dx^{2}}(x)=\frac{d}{dx}(\frac{dy}{dx}(x))$. So, we have:
            \begin{align*}
                \frac{d^{2}y}{dx^{2}}(x)&=\frac{d}{dx}\big(\frac{dy}{dx}\big)=\frac{d}{dx}\big(\frac{d}{dx}(\sin^{-1}(2x))\big)=\frac{d}{dx}\big(\frac{1}{\sqrt{1-4x^{2}}}\frac{d}{dx}(2x)\big)=\frac{d}{dx}\big(\frac{2}{\sqrt{1-4x^{2}}}\big)\\
                &=2\frac{d}{dx}((1-4x^{2})^{-\frac{1}{2}})=-(1-4x^{2})^{-\frac{3}{2}}\frac{d}{dx}(1-4x^{2})=8x(1-4x^{2})^{-\frac{3}{2}}=\frac{8x}{(1-4x^{2})^{\frac{3}{2}}}
            \end{align*}
            \end{proof}
            \begin{problem}
            Let $f(x)=-3x^{4}+4x^{3}$
            \begin{enumerate}
                \item Find the critical points of $f$.
                \item Find the intervals for which $f$ is increasing and decreasing.
                \item Find possible inflection points of $f$.
                \item Find the intervals on which the function is concave up and down.
            \end{enumerate}
            \end{problem}
            \begin{proof}[Solution]
            \
            \begin{enumerate}
                \item Critical points occur when $f'(x)=0$. We have $f'(x)=-12x^{3}+12x^{2}$. Solving for $f'(x)=0$, we have $-12x^{3}+12x^{2}=0 \Rightarrow x^{2}(1-x)=0$. This occurs only when $x=0$ or $x=1$. 
                \item $f$ is increasing when $f'(x)>0$. Solving for this, we have $x^{2}(1-x)>0\Rightarrow x<1$. $f$ is decreasing when $f'(x)<0$, which occurs when $x>1$.
                \item Possible inflection points occur when $f''(x)=0$. Solving for this, we have $f''(x) = -36x^{2}+24x = -12x^{2}(3x-2)$. So $f''(x)=0$ when $x=0$ and when $x=\frac{2}{3}$.
                \item $f$ is concave up when $f''(x)>0$ and concave down when $f''(x)<0$. If $x>0$, then $-12x<0$, so $-12x(3x-2)>0\Rightarrow 3x-2<0$. So $0<x<\frac{2}{3}$. If $x<0$, then $-12x>0$ and $3x-2<0$, and therefore $-12x(3x-2)<0$. If $x>\frac{2}{3}$, then $(3x-2)>0$ and $-12x<0$, so $-12x(3x-2)<0$. Thus, $f$ is concave up on $(0,\frac{2}{3})$ and concanve down on $(-\infty,0)\cup(\frac{2}{3},\infty)$
            \end{enumerate}
            \end{proof}
            \begin{problem}
            Find the equation of the line tangent to the graph of $x+\sqrt{xy}=6$ at the point $(4,1)$.
            \end{problem}
            \begin{proof}[Solution]
            The tangent line is $y=m(x-x_{0})+y_{0}$, where $m$ is the derivative of the graph at $(x_{0},y_{0})$. We have $x_{0}=4$ and $y_{0}=1$. From $\sqrt{xy}=6-x$, and $y=\frac{(6-x)^{2}}{x}$, we have:
            \begin{equation*}
                \frac{d}{dx}(x+\sqrt{xy})=\frac{d}{dx}(6)=0\Rightarrow 1+\frac{1}{2\sqrt{xy}}(y+x\frac{dy}{dx})=0\Rightarrow\frac{dy}{dx}=-\frac{2\sqrt{xy}}{x}-\frac{y}{x}=-\frac{2(6-x)}{x}-\frac{(6-x)^{2}}{x^{2}}
            \end{equation*}
            Evaluating at $x=4$, we get $m=-\frac{5}{4}$. The line is $y=-\frac{5}{4}(x-4)+1$
            \end{proof}
            \begin{problem}
            Compute the second derivative of $y(x)x^{2}\cos(-x)$.
            \end{problem}
            \begin{proof}[Solution]
            First, $\cos(-x)=\cos(x)$, so we can simplify. We have:
            \begin{equation*}
                \frac{dy}{dx}(x)=\frac{d}{dx}(x^{2}\cos(x))=2x\cos(x)-x^{2}\sin(x)\Rightarrow\frac{d^{2}y}{dx^{2}}=2\cos(x)-2x\sin(x)-2x\sin(x)-x^{2}\cos(x)
            \end{equation*}
            Simplifying, we have $\frac{d^{2}y}{dx^{2}}=(2-x^{2})\cos(x)-4x\sin(x)$
            \end{proof}
            \begin{problem}
            Find the extreme values (Global and Relative) of $f(x)=4x^{2}-4x+1$ for $0\leq x\leq 1$.
            \end{problem}
            \begin{proof}[Solution]
            Extreme values occur either at endpoints, or when $f'(x)=0$. $f'(x)=8x-4$. So $f'(x)=0$ when $x=\frac{1}{2}$. At this point, $f(\frac{1}{2})=0$. At the endpoints, $f(0)=1$ and $f(1)=1$, so $x=\frac{1}{2}$ is a global minimum. $x=0$ and $x=1$ are relative maxmima.
            \end{proof}
            \begin{problem}
            Compute the derivative of $g(t)=(t^{3}-2)^{\tan(t)}$
            \end{problem}
            \begin{proof}[Solution]
            Let $y(t)=\ln(g(t))$. Then $\frac{dy}{dt}(t)=\frac{d}{dt}(\tan(t)\ln(t^{3}-2))=\sec^{2}(t)\ln(t^{3}-2)+\tan(t)\frac{3t^{2}}{t^{3}-2}$. But $\frac{dy}{dt}(t)=\frac{d}{dt}(\ln(g(t)))=\frac{1}{g(t)}\frac{dg}{dt}(t)$. So $\frac{dg}{dt}(t)=(t^{3}-2)^{\tan(t)}(\sec^{2}(t)\ln(t^{3}-2)+\tan(t)\frac{3t^{2}}{t^{3}-2})$
            \end{proof}
\end{document}