\documentclass[crop=false,class=article,oneside]{standalone}
%----------------------------Preamble-------------------------------%
\input{../../../preamble.tex}
%----------------------------GLOSSARY-------------------------------%
\makeglossaries
\loadglsentries{../../../glossary}
\loadglsentries{../../../acronym}
%--------------------------Main Document----------------------------%
\begin{document}
    \ifx\ifemagi\undefined
        \section*{Electromagnetism I}
        \setcounter{section}{11}
        \renewcommand\thesubfigure{%
            \arabic{section}.\arabic{figure}.\arabic{subfigure}%
        }
    \fi 
    \subsection{Homework XI}
        \subsubsection{Wangsness 12-3}
        $\mathbf{J} = \rho \mathbf{v}$. $\rho = \frac{Q}{\frac{4}{3}\pi a^3} = \frac{3q}{4\pi a^3}$. $\mathbf{u} = \mathbf{\omega}\times\mathbf{r} = \omega \hat{\mathbf{z}} \times r \hat{\mathbf{r}} = \omega r \sin(\theta) \hat{\boldsymbol{\upvarphi}}$. So, we have that $\mathbf{J} = \frac{3Q}{4\pi a^3} \omega r \sin(\theta) \hat{\boldsymbol{\upvarphi}}$. $\mathbf{da} = rdrd\theta \hat{\boldsymbol{\upvarphi}}$, so $I = \int \mathbf{J} \cdot \mathbf{da} = \frac{3Q \omega}{4\pi a^3} \int_{0}^{\pi} \int_{0}^{a} r^2\sin(\theta)drd\theta = \frac{Q\omega}{2\pi}$
        \subsubsection{Wangsness 13-4}
        We will calculate the force exerted by $C'$ on $C$. $\mathbf{F}_{C'\rightarrow C} = \frac{\mu_0}{4\pi} \oint_{C} \oint_{C'} \frac{I \mathbf{d\ell}\times (I' \mathbf{d\ell}'\times \hat{\mathbf{r}})}{R^2}$. We use the $BAC-CAB$ rule: $\mathbf{A}\times(\mathbf{B}\times \mathbf{C}) = \mathbf{B}(\mathbf{A}\cdot \mathbf{C}) - \mathbf{C}(\mathbf{A}\cdot \mathbf{B})$. We can rewrite the previous integral as  $\mathbf{F}_{C'\rightarrow C} = -\frac{\mu_0 II'}{4\pi} \oint_{C} \oint_{C'} \big[ \mathbf{d\ell}'\cdot(\mathbf{d\ell}\times \frac{\hat{\mathbf{r}}}{R^2}) - \frac{\hat{\mathbf{r}}}{R^2} \mathbf{d\ell}\cdot \mathbf{d\ell}\big]$. Recall that $\nabla(\frac{1}{R}) = \frac{\hat{\mathbf{r}}}{R^2}$. Using this, we have $\mathbf{F}_{C'\rightarrow C} = -\frac{\mu_0 II'}{4\pi} \oint_{C}\oint_{C'} \mathbf{d\ell'}\big[ \mathbf{d\ell}\cdot \nabla(\frac{1}{R})- \frac{\hat{\mathbf{r}}}{R^2} \mathbf{d\ell'} \cdot \mathbf{d\ell}\big]$. From the fundamental theorem of gradients, $\oint \nabla(f) \cdot \mathbf{d\ell} = 0$ for any function $f$. Thus $\oint \nabla(\frac{1}{R}) \cdot \mathbf{d\ell} = 0$. From this we have $\mathbf{F}_{C\rightarrow C'} = -\frac{\mu_0 II'}{4\pi} \oint_{C}\oint_{C'} \frac{\hat{\mathbf{r}}}{R^2} \mathbf{d\ell}'\cdot \mathbf{d\ell}$. We now compute this integral along all four paths of the problem. $\mathbf{d\ell}' = dz' \hat{\mathbf{z}}$ for all paths. Along path $I$, $\mathbf{r} = \hat{\mathbf{x}}d+\hat{\mathbf{z}}z$, $\mathbf{d\ell} = \hat{\mathbf{z}}dz$. Along path $III$, $\mathbf{r} = \hat{\mathbf{x}}(a+d)+\hat{\mathbf{z}}z$, $\mathbf{d\ell} = \hat{\mathbf{z}}dz$. Along paths $II$ and $IV$, $\mathbf{d\ell}\cdot \mathbf{d\ell}' = 0$. Piecing this together, $\mathbf{F}_{C\rightarrow C'} = -\frac{\mu_0 II'}{4\pi}\int_{0}^{b} \int_{-\infty}^{\infty} \frac{\hat{\mathbf{x}}d+\hat{\mathbf{z}}(z-z')}{\big(d^2+(z-z')^2\big)^{3/2}}dz'dz - \frac{\mu_0 II'}{4\pi} \int_{b}^{0} \int_{-\infty}^{\infty} \frac{\hat{\mathbf{x}}(d+a)+\hat{\mathbf{z}}(z-z')}{\big((d+a)^2+(z-z')^2\big)^{3/2}}dz'dz$. Making the substitution $t=z'-z$, we get an integral of the form $\int_{-\infty}^{\infty} \frac{t+z'}{(A+t^2)^{3/2}}dt$. This is an odd function that is integrated over symmetric bounds, and thus the integral is zero. The only part left is the $\hat{\mathbf{x}}$ contribution. Evaluating this integral, we get $\mathbf{F}_{C\rightarrow C'} = -\frac{\mu_0 II' ab}{2\pi d(a+d)}\hat{\mathbf{x}}$.
        \begin{figure}[htbp]
            \centering
            {\includegraphics[scale=0.4]{13-4.png}}
            \caption{Drawing for Wangsness 13-4}
        \end{figure}
        \subsubsection{Wangsness 14-7}
        $\mathbf{R} = \mathbf{r}-\mathbf{r}'$, where $\mathbf{r} = z\hat{\mathbf{z}}$ and $\mathbf{r}' = a\cos(\phi')\hat{\mathbf{x}}+a\sin(\phi')\hat{\mathbf{y}}$. We have $\boldsymbol{d\ell}' = ad\varphi' \hat{\boldsymbol{\upvarphi}}$. Putting this together, we have $\mathbf{R} = z\hat{\mathbf{z}} - a(\cos(\phi')\hat{\mathbf{x}}+\sin(\phi')\hat{\mathbf{y}})$. So:
        \begin{align*}
            \mathbf{B} &= \frac{\mu_0 I'}{4\pi}\int \frac{\boldsymbol{d\ell}\times \mathbf{R}}{R^3} = \frac{\mu_0I'}{4\pi} \int_{-\alpha}^{\alpha} \frac{ad\phi' \hat{\boldsymbol{\upvarphi}}\times (z\hat{\mathbf{z}}-a\cos(\phi')\hat{\mathbf{x}}-a\sin(\phi')\hat{\mathbf{y}})}{(z^2+a^2)^{3/2}}\\
            &= \frac{\mu_0 I'a}{4\pi(z^2+a^2)^{3/2}}\int_{-\alpha}^{\alpha} (-\sin(\phi')\hat{\mathbf{x}}+\cos(\phi')\hat{\mathbf{y}})\times (-a\cos(\phi')\hat{\mathbf{x}}-a\sin(\phi')\hat{\mathbf{y}}+z\hat{\mathbf{z}})d\phi'\\
            &= \frac{\mu_0 I'a}{4\pi (z^2+a^2)^{3/2}}\int_{-\alpha}^{\alpha} (z\cos(\phi')\hat{\mathbf{x}}+z\sin(\phi')\hat{\mathbf{y}}+a\hat{\mathbf{z}})d\phi'
        \end{align*}
        Sine is an odd function, and the limit is over a symmetric interval, and thus the $\hat{\mathbf{y}}$ component is zero. So we have:
        \begin{equation*}
            \mathbf{B} = \frac{\mu_0 I' a}{2\pi (z^2+a^2)^{3/2}}\big(z\sin(\alpha)\hat{\mathbf{x}}+a\alpha \hat{\mathbf{z}}\big)    
        \end{equation*}
        \subsubsection{Wangsness 14-15}
        The force on $q$ is given by $\mathbf{F} = q\mathbf{v}\times \mathbf{B}$. We first get $\mathbf{B}$ at $q$. $\mathbf{B} = \frac{\mu_0}{4\pi} \int \frac{I' d\ell' \times \hat{\mathbf{r}}}{R^2}$. For this problem, $\mathbf{R} = -\rho' \hat{\boldsymbol{\uprho}}$. We need only compute the integral along paths $I$ and $III$, for along $II$ and $IV$ we have that $\mathbf{d\ell}$ and $\mathbf{R}$ are parallel. So, we have $\mathbf{B} = \frac{\mu_0}{4\pi} \int_{0}^{\pi} \frac{I'(-ad\phi' \hat{\boldsymbol{\upvarphi}})\times (-a\hat{\boldsymbol{\uprho}})}{a^3}+ \frac{\mu_0}{4\pi} \int_{0}^{\pi} \frac{I'(bd\phi' \hat{\boldsymbol{\upvarphi}})\times (-b\hat{\boldsymbol{\uprho}})}{b^3} = \frac{\mu_0 I'}{4} \frac{b-a}{ab} \hat{\mathbf{z}}$. The force is $\mathbf{F} = qv\hat{\mathbf{y}} \times \frac{\mu_0 I}{4} \frac{b-a}{ab} \hat{\mathbf{z}} = \frac{qv\mu_0 I'}{4} \frac{b-a}{ab} \hat{\mathbf{x}}$
        \begin{figure}[htbp]
            \centering
            {\includegraphics[scale=0.4]{14-15.png}}
            \caption{Drawing for Wangsness 14-15}
        \end{figure}
\end{document}