\documentclass[crop=false,class=article,oneside]{standalone}
%----------------------------Preamble-------------------------------%
\input{../../../preamble.tex}
%----------------------------GLOSSARY-------------------------------%
\makeglossaries
\loadglsentries{../../../glossary}
\loadglsentries{../../../acronym}
%--------------------------Main Document----------------------------%
\begin{document}
    \ifx\ifphysicscourseselectromagnetismI\undefined
        \section*{Electromagnetism I}
        \setcounter{section}{6}
        \renewcommand\thesubfigure{%
            \arabic{section}.\arabic{figure}.\arabic{subfigure}%
        }
    \fi
    \subsection{Homework VI}
    \subsubsection{Wangsness 5-1}
    $\mathbf{E} = (yz-2x)\hat{\mathbf{x}}+xz\hat{\mathbf{y}}+xy\hat{\mathbf{z}}$. So, $\nabla \times \mathbf{E} = (x-x)\hat{\mathbf{x}}-(y-y)\hat{\mathbf{y}}+(z-z)\hat{\mathbf{z}} = \mathbf{0}$. Therefore $\mathbf{E}$ is a possible electrostatic field. Indeed, writen $\mathbf{E} = \nabla(\phi)$, we get $-\frac{\partial \phi}{\partial x} = yz-2x$, so $-\phi = xyz - x^2 + g(y,z)$, where $g$ is a function of $y$ and $z$ (Note: $\frac{\partial g}{\partial x} = 0$ as $g$ is not a function of $x$). Now $-\frac{\partial \phi}{\partial y} = xz$ and $-\frac{\partial \phi}{\partial z} = xy$, and thus $g(y,z) = constant$. So, $\phi(x,y,z) = -xyz+x^2 + C$, where $C$ is some constant. We may choose $C$ is we desire, so let $C=0$ to make things easy. The integral $\int \mathbf{E}\cdot \mathbf{d\ell}$ from the origin $(0,0,0)$ to a point $(x,y,z)$ is thus independent of path and may be computed by using the fundamental theorem of gradients. That is, $\int \mathbf{E}\cdot \mathbf{d\ell} = -\int _{(0,0,0)}^{(x,y,z)} \nabla(\phi)\cdot \mathbf{d\ell} = -\big(\phi(x,y,z) -\phi(0,0,0)\big) = \phi(0,0,0)-\phi(x,y,z)$. Now, $\phi(0,0,0)= 0$, and thus $\int_{(0,0,0)}^{(x,y,z)}\mathbf{E}\cdot \mathbf{d\ell} = -\phi(x,y,z) = xyz-x^2$.
    \subsubsection{Wangsness 5-3}
    $\phi = \frac{1}{4\pi \epsilon_0}\big[ \frac{q}{R_{+}} - \frac{q}{R_{-}}\big] = \frac{q}{4\pi \epsilon_0}\big[\frac{1}{\sqrt{x^2+y^2+(z-a)^2}}-\frac{1}{\sqrt{x^2+y^2+(z+a)^2}}\big]$. At $z=0$, we get $\phi = \frac{q}{4\pi \epsilon_0}\big[ \frac{1}{\sqrt{x^2+y^2+a^2}}-\frac{1}{\sqrt{x^2+y^2+a^2}}\big] = 0$. Thus, the entire $xy-$plane is an equipotential surface with $\phi = 0$.
    \begin{figure}[htbp]
      \centering
        {\includegraphics[scale=0.4]{5-3.png}}
        \caption{Drawing for Wangsness 5-3}
    \end{figure}
    \subsubsection{Wangsness 5-4}
    $\phi = \frac{1}{4\pi \epsilon_0} \sum \frac{q_i}{R_i} = \frac{1}{4\pi \epsilon_0}\bigg[ \frac{q}{\sqrt{a^2/4}}+\frac{2q}{\sqrt{a^2/2}}-\frac{4q}{\sqrt{a^2/2}}+\frac{3q}{\sqrt{a^2/2}}\bigg] = \frac{q}{\sqrt{2}\pi \epsilon_0 a}$. To know $\mathbf{E}$ from $\phi$, $\phi$ must be known in some region about the point, not just at the point. To be precise in mathematical terms, we must know $\phi$ in some open set about the point in order to compute $\nabla(\phi)$. This is analogous to functions in calculus. Suppose $f$ is a function and $a$ is a real number, and suppose we know the value of $f(a)$. Can we determine what $f'(a)$ is? The answer is no, there is not enough information. If we know what $f(x)$ is in some interval $(a-\epsilon,a+\epsilon)$, then we can compute $f'(a)$.
    \begin{figure}[htbp]
        \centering
        {\includegraphics[scale=0.4]{5-4.png}}
        \caption{Drawing for Wangsness 5-4}
    \end{figure}
    \subsubsection{Wangsness 5-10}
    We know that $\mathbf{E} = \begin{cases} \frac{2A a^{7/2}}{7\epsilon_0 r^2}\hat{\mathbf{r}}, & r>a \\ \frac{2A r^{3/2}}{7\epsilon_0}, & r<a\end{cases}$. So, $\Delta \phi = \int \mathbf{E} \cdot \mathbf{d\ell}$. Now, $\mathbf{d\ell} = -dr(-\hat{\mathbf{r}}) = \mathbf{dr}$. We split the integral into two parts and compute: $\int \mathbf{E}\cdot \mathbf{d\ell} = \int_{0}^{a} \mathbf{E}\cdot \mathbf{dr} + \int_{a}^{\infty} \mathbf{E}\cdot \mathbf{dr} = \frac{4A a^{5/4}}{35 \epsilon_0}\bigg[ \frac{7}{2}-\big(\frac{r}{a}\big)^{7/2}\bigg]$.
    \subsubsection{Wangsness 5-11}
    We have that $\mathbf{E} = \begin{cases} \mathbf{0}, & r<a\\ \frac{Q}{4\pi \epsilon_0}\bigg(\frac{r^3-a^3}{b^3-a^3}\bigg)\hat{\mathbf{r}}, & a\leq r \leq b\\ \frac{Q}{4\pi \epsilon_0 r^2}\hat{\mathbf{r}}, & r>b\end{cases}$ We thus split the integral into three regions and compute: $\Delta\phi=\int \mathbf{E}\cdot \mathbf{d\ell} = \int_{0}^{a} \mathbf{E}\cdot \mathbf{dr}+\int_{a}^{b} \mathbf{E}\cdot \mathbf{dr}+\int_{b}^{\infty} \mathbf{E}\cdot \mathbf{dr}$. We then obtain $\phi(\mathbf{r}) = \begin{cases} \frac{\rho_c(b^3-a^3)}{3\epsilon_0 r}, & r>b \\ \frac{\rho}{3\epsilon_0}\bigg[ \frac{3}{2}b^2-\frac{r^2}{2}-\frac{a^3}{r}\bigg], & a\leq r \leq b\\ \frac{\rho_c}{2\epsilon_0}(b^2-a^2), & r<a\end{cases}$
    \subsubsection{Wangsness 5-14}
    $\phi = \frac{1}{4\pi \epsilon_0}\iint \frac{\sigma_c da'}{R}$. Here, $R = |\mathbf{r}-\mathbf{r}'| = \sqrt{a^2+r^2-2ar\cos(\theta')}$, and $da' = a^2\sin(\theta')d\theta'd\phi'$. So, we have $\phi = \frac{\sigma_c}{4\pi \epsilon_0}\int_{0}^{2\pi}\int_{0}^{\pi} \frac{a^2\sin(\theta')d\theta' d\phi'}{\sqrt{a^2+r^2-2ar\cos(\theta')}} = \frac{\sigma_c a^2}{2\epsilon_0}\int_{0}^{\pi} \frac{\sin(\theta')d\theta'}{\sqrt{a^2-r^2-2ar\cos(\theta')}}$. Let $u = \cos(\theta')$. Then $du = -\sin(\theta')d\theta'$, and we have $-\int\frac{du}{\sqrt{a^2+r^2-2aru}}$. Note that $r$ and $a$ are constants in the integral, and thus this can be computed by trigonometric substitution (Or wolframalpha/integral tables if you're lazy). We thus have $\phi(\mathbf{r}) = \begin{cases}\frac{a^2\sigma}{\epsilon_0 r}, & r>a \\ \frac{a\sigma}{\epsilon_0}, & r<a\end{cases}$.
\end{document}