\documentclass[crop=false,class=book,oneside]{standalone}                      %
%----------------------------------Preamble------------------------------------%
\input{../../preamble.tex}                                                     %
                                                                               %
% Add tikz files to the file path.                                             %
\makeatletter                                                                  %
    \def\input@path{{../../tikz/}}                                             %
\makeatother                                                                   %
%----------------------------------GLOSSARY------------------------------------%
\makeglossaries                                                                %
\loadglsentries{../../glossary}                                                %
\loadglsentries{../../acronym}                                                 %
%--------------------------------Main Document---------------------------------%
\begin{document}
    \title{Linear and Quadratic Equations}
    \author{\vspace{-5ex}}
    \date{\vspace{-5ex}}
    \maketitle
    \setcounter{chapter}{1}
    \section{Problems with Linear Equations}
        \begin{problem}
            Given the following two points in the plane,
            graph the line that passes through these, compute
            the slope and $y$ intercept, and find the root.
            Then give the equation of the line in slope-intercept
            form.
            \begin{enumerate}
                \begin{multicols}{3}
                    \item $(0,0)$, $(1,1)$
                    \item $(2,3)$, $(\minus{1},\minus{2})$
                    \item $(2,0)$, $(3,1)$
                    \item $(\minus{1},\minus{2})$, $(\frac{1}{2},2)$
                    \item $(1,1)$, $(3,1)$
                    \item $(\frac{3}{4},\frac{2}{3})$, $(\frac{5}{2},2)$
                    \item $(\sqrt{2},\sqrt{3})$, $(\sqrt{8},\sqrt{12})$
                    \item $(0,\pi)$, $(\minus{1},0)$
                    \item $(1,2)$, $(1,3)$
                \end{multicols}
            \end{enumerate}
        \end{problem}
        \begin{solution}
            Given $(x_{1},y_{1})$ and $(x_{2},y_{2})$, we can compute the
            slope of the line through these two points as follows:
            \begin{equation}
                m=\frac{y_{2}-y_{1}}{x_{2}-x_{1}}
            \end{equation}
            Once this is done, we have $y=mx+b$. To compute for $b$ we simply
            plug in either $x_{1}$ and $y_{1}$, or $x_{2}$ and $y_{2}$, and
            then solve for $b$. That is:
            \begin{equation}
                y_{1}=mx_{1}+b
                \quad\Longrightarrow\quad
                y_{1}-mx_{1}=b
            \end{equation}
            Using our equation for $m$, we obtain:
            \begingroup
                \addtolength{\jot}{0.5em}
                \begin{subequations}
                    \begin{align}
                        y_{1}-mx_{1}
                        &=y_{1}-\frac{y_{2}-y_{1}}{x_{2}-x_{1}}x_{1}\\
                        &=y_{1}\frac{x_{2}-x_{1}}{x_{2}-x_{1}}-
                               \frac{y_{2}-y_{1}}{x_{2}-x_{1}}x_{1}\\
                        &=\frac{y_{1}(x_{2}-x_{1})-x_{1}(y_{2}-y_{1})}
                               {x_{2}-x_{1}}\\
                        &=\frac{y_{1}x_{2}-y_{1}x_{1}-y_{2}x_{1}+y_{1}x_{1}}
                               {x_{2}-x_{1}}\\
                        &=\frac{y_{1}x_{2}-y_{2}x_{1}}{x_{2}-x_{1}}
                    \end{align}
                \end{subequations}
            \endgroup
            We can repeat this $y_{2}$ and $x_{2}$, to obtain:
            \begingroup
                \addtolength{\jot}{0.5em}
                \begin{subequations}
                    \begin{align}
                        y_{2}-mx_{2}
                        &=y_{2}-\frac{y_{2}-y_{1}}{x_{2}-x_{1}}x_{2}\\
                        &=y_{2}\frac{x_{2}-x_{1}}{x_{2}-x_{1}}-
                               \frac{y_{2}-y_{1}}{x_{2}-x_{1}}x_{2}\\
                        &=\frac{y_{2}(x_{2}-x_{1})-x_{2}(y_{2}-y_{1})}
                               {x_{2}-x_{1}}\\
                        &=\frac{y_{2}x_{2}-y_{2}x_{1}-y_{2}x_{2}+y_{1}x_{2}}
                               {x_{2}-x_{1}}\\
                        &=\frac{y_{1}x_{2}-y_{2}x_{1}}{x_{2}-x_{1}}
                    \end{align}
                \end{subequations}
            \endgroup
            Piecing this together, we have found that:
            \begin{equation}
                b=y_{1}-mx_{1}
                 =\frac{y_{1}x_{2}-y_{2}x_{1}}{x_{2}-x_{2}}
                 =y_{2}-mx_{2}
            \end{equation}
            And thus it doesn't matter which point we choose when calculating
            $b$. Computing for the points $(0,0)$ and $(1,1)$, we have:
            \begin{equation}
                m=\frac{1-0}{1-0}=\frac{1}{1}=1
            \end{equation}
            So the line is of the form $y=x+b$. To determine the $y$ intercept,
            we simply plug in either $(x_{1},y_{1})$ or $(x_{2},y_{2})$ and
            solve for $b$. Let's use the point $(0,0)$ since it will make the
            arithmetic easier. We have:
            \begin{equation}
                0=1(0)+b
                \quad\Longrightarrow\quad
                b=0
            \end{equation}
            The equation of the line through $(0,0)$ and $(1,1)$ is thus
            $y=x$. The slope is 1 and the $y$ intercept is zero. The root
            of $y=mx+b$ is when $y=0$. Equivalently, this is when
            $mx+b=0$. For the line $y=x$, this occurs when $x=0$.
            \par\hfill\par
            For the points $(2,3)$ and $(\minus{1},\minus{2})$, we can again
            compute the slope and obtain:
            \begin{equation}
                m=\frac{3-(\minus{2})}{2-(\minus{1})}
            \end{equation}
            Recall that subtracting a negative number is the same thing as
            adding a positive number, so we have:
            \begin{equation}
                m=\frac{3-(\minus{2})}{2-(\minus{1})}
                 =\frac{3+2}{2+1}
                 =\frac{5}{3}
            \end{equation}
            To compute the $y$ intercept, we can simply plug in $x=2$ and $y=3$:
            \begin{equation}
                3=\frac{5}{3}(2)+b
                \quad\Longrightarrow\quad
                3=\frac{10}{3}+b
                \quad\Longrightarrow\quad
                3-\frac{10}{3}=b
            \end{equation}
            To simplify, we need to rewrite this in a manner such that the
            denominators of the two are equal. We get:
            \begin{equation}
                3-\frac{10}{3}=b
                \quad\Longrightarrow\quad
                \frac{9}{3}-\frac{10}{3}=b
                \quad\Longrightarrow
                \frac{9-10}{3}=b
            \end{equation}
            Carring out this subtraction, we obtain $b=\minus{1}/3$. The
            slope-intercept form is thus:
            \begin{equation}
                y=\frac{5}{3}x-\frac{1}{3}
                \quad\Longrightarrow\quad
                y=\frac{5x-1}{3}
            \end{equation}
            This simplified version on the right makes it simple to compute the
            root of this line. The root occurs when $y=0$. This can only happen
            if $5x-1=0$. Thus we see that the root is at $x=1/5$.
            \begin{figure}
                \centering
                \captionsetup{type=figure}
                \begin{subfigure}[b]{0.49\textwidth}
                    \centering
                    \resizebox{\textwidth}{!}{%
                        \subimport{tikz/}{Linear_Equation_Example_001.tex}}
                    \subcaption{Graph of $y=x$}
                \end{subfigure}
                \begin{subfigure}[b]{0.49\textwidth}
                    \centering
                    \resizebox{\textwidth}{!}{%
                        \subimport{tikz/}{Linear_Equation_Example_002.tex}}
                    \subcaption{Graph of $y=\frac{5}{3}x-\frac{1}{3}$}
                \end{subfigure}
                \caption{Solutions to the First Two Problems.}
                \label{fig:Solutions_to_First_Two_Problems}
            \end{figure}
            Next, for $(2,0)$ and $(3,1)$ we can continue with
            the same method as before.
            \begin{equation}
                m=\frac{3-2}{1-0}
                 =1
            \end{equation}
            The line is thus $y=x+b$. Solving for $b$, we get:
            \begin{equation}
                0=2+b
                \quad\Longrightarrow\quad
                b=\minus{2}
            \end{equation}
            The equation is $y=x-2$. The root then occurs when $x=2$.
        \end{solution}
        \newpage
        \begin{problem}
            The general equation for a line is:
            \begin{equation}
                \label{eqn:general_line}%
                Ax+By+C=0
            \end{equation}
            This is contrasted with the slope-intercept form:
            \begin{equation}
                \label{eqn:slope_intercept_form}%
                y=mx+b
            \end{equation}
            Find an example of a line that can be written
            in the form of Eqn.~\ref{eqn:general_line} but
            cannot be written in the form of
            Eqn.~\ref{eqn:slope_intercept_form}. Draw the graph of
            this line.
            \par
            Hint: Consider the line the passes through
            $(1,1)$ and $(3,1)$. What's special about this line?
            Can it be written in the form of
            Eqn.~\ref{eqn:general_line}? What about
            Eqn.~\ref{eqn:slope_intercept_form}?
        \end{problem}
        \begin{solution}
            \begin{align}
                Ax+By+C&=0\\
                \Rightarrow{B}y&=\minus{A}x-C\\
                \Rightarrow{y}&=\minus\frac{A}{B}x-\frac{C}{B}\\
                \Rightarrow{m}&=\minus\frac{A}{B}\\
                \Rightarrow{b}&=\minus\frac{C}{B}
            \end{align}
        \end{solution}
        \newpage
        \begin{problem}
            Solve the following systems of linear equations.
            Determine if there is one solution, infinitely many
            solutions, or no solutions. Graph the lines as well.
            \begin{align*}
                (1)\quad{y}&=3x+2&(2)\quad{3}y&=6x+6\\
                2y&=4x+8&y&=2x+2\\
                \hfill\\
                (3)\quad{2}y&=3x+3&(4)\quad{2}y&=2x+1\\
                4y&=6x+7&3y&=x-6
            \end{align*}
        \end{problem}
        \begin{align*}
            2y-3x&=3\\
            4y-6x&=7
        \end{align*}
        \par\hfill\par
        \begin{align*}
            \minus{3}x+2y&=3\\
            \minus{6}x+4y&=7
        \end{align*}
        \par\hfill\par
        \begin{equation}
            \begin{pmatrix}
                \minus{3}&2\\
                \minus{6}&4
            \end{pmatrix}
            \begin{pmatrix}
                x\\y
            \end{pmatrix}
            =
            \begin{pmatrix}
                3\\7
            \end{pmatrix}
        \end{equation}
        \begin{equation}
            \begin{pmatrix}
                x\\y
            \end{pmatrix}
            =
            \begin{pmatrix}
                a&b\\
                c&d
            \end{pmatrix}
            \begin{pmatrix}
                3\\7
            \end{pmatrix}
        \end{equation}
        \begin{equation}
            \begin{bmatrix}
                \minus{3}&2&\vline&1&0\\
                \minus{6}&4&\vline&0&1
            \end{bmatrix}
        \end{equation}
\end{document}