\documentclass[crop=false,class=book]{standalone}
%---------------PREAMBLE------------%
\input{../../preamble.tex}
%---------------GLOSSARY------------%
\makeglossaries
\loadglsentries{../../glossary}
\loadglsentries{../../acronym}
%--------------Title Page-----------%
\begin{document}
\chapter{Calculus II}
\section{Exams}
\subsection{Practice Exam I}
\begin{problem}
Use the Midpoint Rule to estimate the area under the graph of $f(x)=16-x^{2}$ between $x=-4$ and $x=4$ using four rectangles. Estimate the average of $f$ on the same interval.
\end{problem}
\begin{proof}[Solution]
\
\begin{table}[H]
    \centering
    \begin{tabular}{|c|c|c|c|}
        \hline
        Start&End&\# Pts&$\Delta x$\\
        \hline
        $a=-4$&$b=4$&$n=4$&$\frac{b-a}{n}=2$\\
        \hline
    \end{tabular}
\end{table}
The midpoints are $m_{n}=\frac{x_{n-1}+x_{n}}{2}$, where $x_{0}=a$, and $x_{n}=x_{n-1}+\Delta x$.
\begin{table}[H]
    \centering
    \begin{tabular}{|c|c|c|c|}
        \hline
        $m_{1}$&$m_{2}$&$m_{3}$&$m_{4}$\\
        \hline
        $-3$&$-1$&$1$&$3$\\
        \hline
    \end{tabular}
\end{table}
The midpoint rule says $A_{M}=\sum_{k=1}^{n}f(m_{k})\Delta x$
\begin{table}[H]
    \centering
    \begin{tabular}{|c|c|c|c|}
        \hline
        $f(m_{1})$&$f(m_{2})$&$f(m_{3})$&$f(m_{4})$\\
        \hline
        $7$&$15$&$15$&$7$\\
        \hline
    \end{tabular}
\end{table}
So, $A_{M}=2(7+15+15+7)=2(44)=88$. The estimated average of $f$ is $\frac{A_{m}}{b-a}=\frac{88}{8}=11$
\end{proof}
\begin{problem}
Using the Fundamental Theorem of Calculus, find $\frac{dy}{dx}$:
\begin{enumerate}
    \begin{multicols}{2}
        \item $y=\int_{\sin(x)}^{0}\frac{4dt}{\sqrt{1-t^{2}}}$
        \item $y=\int_{3+x^{2}}^{6}\frac{t}{1+e^{t}}dt$
    \end{multicols}
\end{enumerate}
\end{problem}
\begin{proof}[Solution]
\
\begin{enumerate}
    \item   \begin{align*}
    y&=\int_{\sin(x)}^{0}\frac{4dt}{\sqrt{1-t^{2}}}=-\int_{0}^{\sin(x)}\frac{4dt}{\sqrt{1-t^{2}}}\Rightarrow\frac{dy}{dx}=-\frac{d}{dx}\int_{0}^{\sin(x)}\frac{4dt}{\sqrt{1-t^{2}}}\\
    \Rightarrow\frac{dy}{dx}&=-\frac{4}{\sqrt{1-\sin^{2}(x)}}\frac{d}{dx}(\sin(x))=-\frac{4\cos(x)}{|\cos(x)|}=-4\sgn(x)
            \end{align*}
    \item   \begin{align*}
    y&=\int_{3+x^{2}}^{6}\frac{t}{1+e^{t}}dt=-\int_{6}^{3+x^{2}}\frac{t}{1+e^{t}}dt\Rightarrow\frac{dy}{dx}=-\frac{d}{dx}\int_{6}^{3+x^{2}}\frac{t}{1+e^{t}}dt\\
    &=-\frac{3+x^{2}}{1+e^{3+x^{2}}}\frac{d}{dx}(3+x^{2})=-\frac{2x(3+x^{2})}{1+e^{3+x^{2}}}
            \end{align*}
\end{enumerate}
\end{proof}
\newpage
\begin{problem}
Evaluate $\int_{-2}^{2}(x^{2}+e^{2})dx$
\end{problem}
\begin{proof}[Solution]
\begin{equation*}
    \int_{-2}^{2}(x^{2}+e^{2})dx=\frac{1}{3}x^{3}+e^{2}x\big|_{-2}^{2}=\frac{16}{3}+4e^{2}
\end{equation*}
\end{proof}
\begin{problem}
\
\begin{enumerate}
    \begin{multicols}{3}
        \item $\int_{0}^{1}\frac{4x^{3}}{(x^{4}-3)^{2}}dx$
        \item $\int e^{5x}(e^{5x}+4)^{2}dx$
        \item $\int\cos^{3}(3x)\sin(3x)dx$
    \end{multicols}
\end{enumerate}
\end{problem}
\begin{proof}[Solution]
\
\begin{enumerate}
    \item   \begin{align*}
    u=x^{4}-3,du&=4x^{3}dx,x=0\Rightarrow u=-3,x=1\Rightarrow u=-2\\
    \int_{0}^{1}\frac{4x^{3}}{(x^{4}-3)^{2}}dx&=\int_{-3}^{-2}\frac{du}{u^{2}}=-\frac{1}{u}\big|_{-3}^{-2}=\frac{1}{6}
            \end{align*}
    \item   \begin{align*}
    u=e^{5x}+4,du&=5e^{5x}dx\Rightarrow e^{5x}dx=\frac{1}{5}du\\
    \int e^{5x}(e^{5x}+4)^{2}dx&=\frac{1}{5}\int u^{2}du=\frac{1}{15}u^{3}+C=\frac{1}{15}(e^{5x}+4)^{3}+C
            \end{align*}
    \item   \begin{align*}
    u=\cos(3x),du&=-3\sin(3x)dx\Rightarrow -\frac{1}{3}du=\sin(3x)dx\\
    \int \cos^{3}(3x)\sin(3x)dx&=-\frac{1}{3}\int u^{3}du=-\frac{1}{12}u^{4}+C=-\frac{1}{12}\cos^{4}(3x)+C
            \end{align*}
\end{enumerate}
\end{proof}
\begin{problem}
Find the area of the region bounded by the curves $f(x)=-x^{2}+4x-2$ and $g(x)=x^{2}-2$
\end{problem}
\begin{proof}[Solution]
The points of intersection are: $x^{2}-2=-x^{2}+4x-2\Rightarrow 2x(x-2)=0\Rightarrow x=0,x=2$.
The area between the curves is $A=\int_{0}^{2}(f(x)-g(x))dx$:
\begin{equation*}
    A=\int_{0}^{2}(f(x)-g(x))dx=\int_{0}^{2}(-2x^{2}+4x)dx=-\frac{2}{3}x^{3}+2x^{2}\big|_{0}^{2}=\frac{8}{3}
\end{equation*}
\end{proof}
\begin{problem}
Evaluate $\int xe^{2x}dx$
\end{problem}
\begin{proof}[Solution]
\
\begin{table}[H]
    \centering
    \begin{tabular}{|c|c|}
        \hline
        $u=x$&$dv=e^{2x}dx$\\
        \hline
        $du=dx$&$v=\frac{1}{2}e^{2x}$\\
        \hline
    \end{tabular}
\end{table}
\begin{equation*}
    \int udv=uv-\int vdu\Rightarrow \int xe^{2x}dx=\frac{1}{2}xe^{2x}-\frac{1}{2}\int e^{2x}dx=\frac{1}{2}xe^{2x}-\frac{1}{4}e^{2x}+C
\end{equation*}
\end{proof}
\begin{problem}
Evaluate $\int_{0}^{\pi^{2}}\cos(\sqrt{x})dx$
\end{problem}
\begin{proof}[Solution]
Let $y=\sqrt{x}$. $dy=\frac{1}{2\sqrt{x}}dx\Rightarrow dx=2\sqrt{x}dy=2ydy\Rightarrow\int\cos(\sqrt{x})dx=2\int y\cos(y)dy$
\begin{table}[H]
    \centering
    \begin{tabular}{|c|c|}
        \hline
        $u=y$&$dv=\cos(y)dy$\\
        \hline
        $du=dy$&$v=\sin(y)$\\
        \hline
    \end{tabular}
\end{table}
\begin{align*}
    \int\cos(\sqrt{x})dx&=2\int y\cos(y)dy=2\big(y\sin(y)-\int\sin(y)dy\big)=2y\sin(y)+2\cos(y)\\
    \Rightarrow \int_{0}^{\pi^{2}}\cos(\sqrt{x})dx&=2\sqrt{x}\cos(\sqrt{x})+2\cos(\sqrt{x})\big|_{0}^{\pi^{2}}=-4
\end{align*}
\end{proof}
\subsection{Exam I}
\begin{problem}
Using the Fundamental Theorem of Calculus, find $\frac{dy}{dx}$:
\begin{enumerate}
    \begin{multicols}{2}
        \item $y=\int_{\sqrt{x}}^{0}\cos(t^{4})dt$
        \item $y=\int_{5+2x^{2}}^{6}(e^{t}+2t)dt$
    \end{multicols}
\end{enumerate}
\end{problem}
\begin{proof}[Solution]
\
\begin{enumerate}
    \item   \begin{align*}
        y&=\int_{\sqrt{x}}^{0}\cos(t^{4})dt=-\int_{0}^{\sqrt{x}}\cos(t^{4})dt\Rightarrow     \frac{dy}{dx}=-\frac{d}{dx}\int_{0}^{\sqrt{x}}\cos(t^{4})dt\\
        &=\cos(x^{2})\frac{d}{dx}(\sqrt{x})=-\frac{\cos(x^{2})}{2\sqrt{x}}
            \end{align*}
    \item   \begin{align*}
        y&=\int_{5+2x^{2}}^{6}(e^{t}+2t)dt=-\int_{6}^{5+2x^{2}}(e^{t}+2t)dt\Rightarrow \frac{dy}{dx}=-\frac{d}{dx}\int_{6}^{5+2x^{2}}(e^{t}+2t)dt\\
        &=-[e^{5+2x^{2}}+2(5+2x^{2})]\frac{d}{dx}(5+2x^{2})=-4x[e^{5+2x^{2}}+10+4x^{2}]
            \end{align*}
\end{enumerate}
\end{proof}
\begin{problem}
Evaluate the integral: $\int(\frac{3}{x}-\frac{2}{x^{3}}-\sqrt[3]{x}+2e^{2x}+\cos(\pi x)-\pi)dx$
\end{problem}
\begin{proof}[Solution]
$\int(\frac{3}{x}-\frac{2}{x^{3}}-\sqrt[3]{x}+2e^{2x}+\cos(\pi x)-\pi)dx=3\ln(|x|)+\frac{1}{x^{2}}-\frac{3}{4}x^{\frac{4}{3}}+e^{2x}+\frac{\sin(\pi x)}{\pi}-\pi x+C$
\end{proof}
\begin{problem}
Evaluate the following integrals:
\begin{enumerate}
    \begin{multicols}{4}
        \item $\int_{0}^{2}3x^{2}\sqrt{x^{3}+8}dx$
        \item $\int\frac{e^{3y}}{e^{3y}-5)^{2}}dy$
        \item $\int\frac{1}{\arctan^{2}(x)(1+x^{2})}dx$
        \item $\int_{0}^{\pi/4}\sin^{3}(2\theta)\cos(2\theta)d\theta$
    \end{multicols}
\end{enumerate}
\end{problem}
\begin{proof}[Solution]
\
\begin{enumerate}
    \item   \begin{align*}
    u&=x^{3}+8, du=3x^{2}dx\\
    \int 3x^{2}\sqrt{x^{3}+8}dx&=\int\sqrt{u}du=\frac{3}{2}u^{\frac{3}{2}}+C=\frac{3}{2}(x^{3}+8)^{\frac{3}{2}}+C\\
    \Rightarrow\int_{0}^{2}3x^{2}\sqrt{x^{3}+8}dx&=\frac{3}{2}(x^{3}+8)^{\frac{3}{2}}\big|_{0}^{2}=\frac{3}{2}[(2^{2}+8)^{\frac{3}{2}}-(8)^{\frac{3}{2}}]=\frac{32}{3}(4-\sqrt{2})
            \end{align*}
    \item   \begin{align*}
    u&=e^{3y}-5,du=3e^{3y}dy\Rightarrow e^{3y}dy=\frac{1}{3}du\\
    \int\frac{e^{3y}}{(e^{3y}-5)^{3}}dy&=\frac{1}{3}\int\frac{du}{u^{3}}=\frac{1}{3}\int u^{-3}du=-\frac{1}{6}u^{-2}+C=-\frac{1}{6}(e^{3y}-5)^{-2}+C
            \end{align*}
    \item   \begin{align*}
    u&=\arctan(x),du=\frac{1}{1+x^{2}}dx\\
    \int\frac{1}{\arctan^{2}(x)(1+x^{2})}dx&=\int\frac{du}{u^{2}}=-\frac{1}{u}+C=-\frac{1}{\arctan(x)}+C
            \end{align*}
    \item   \begin{align*}
    u=\sin(2\theta),du=2\cos(2\theta)d\theta\Rightarrow\cos(2\theta)d\theta&=\frac{1}{2}du,\theta=0\Rightarrow u=0,\theta=\frac{\pi}{4}\Rightarrow u=1\\
    \int_{0}^{\frac{\pi}{4}}\sin^{3}(2\theta)\cos(2\theta)d\theta&=\frac{1}{2}\int_{0}^{1}u^{3}du=\frac{1}{8}u^{4}\big|_{0}^{1}=\frac{1}{8}
            \end{align*}
\end{enumerate}
\end{proof}
\begin{problem}
FInd the area of the region bounded by the curves of $y=x^{2}+4$ and $y=-x^{2}+6x+4$
\end{problem}
\begin{proof}[Solution]
We first find the points of intersection of the two curves:
\begin{equation*}
    x^{2}+4=-x^{2}+6x+4\Rightarrow2x^{2}-6x=0\Rightarrow 2x(x-3)=0\Rightarrow x=0,x=3
\end{equation*}
The area bounded by $f(x)=-x^{2}+6x+4$ and $g(x)=x^{2}+4$ is $\int_{0}^{3}(f(x)-g(x))dx$
\begin{equation*}
    A=\int_{0}^{3}(f(x)-g(x))dx=\int_{0}^{3}(-2x^{2}+6x)dx=[-\frac{2}{3}+3x^{2}]_{0}^{3}=-\frac{2}{3}(3)^{3}+3(3)^{2}-0=9
\end{equation*}
\end{proof}
\begin{problem}
Evaluate $\int x^{2}e^{3x}dx$
\end{problem}
\begin{proof}[Solution]
\
\begin{table}[H]
    \centering
    \begin{tabular}{|c|c|}
        \hline
        $u=x^{2}$&$dv=e^{3x}dx$\\
        \hline
        $du=2xdx$&$v=\frac{1}{3}e^{3x}$\\
        \hline
    \end{tabular}
\end{table}
\begin{equation*}
    \int udv=uv-\int vdu\Rightarrow \int x^{2}e^{3x}dx=\frac{1}{3}x^{2}e^{3x}-\frac{2}{3}\int xe^{3x}dx
\end{equation*}
\begin{table}[H]
    \centering
    \begin{tabular}{|c|c|}
        \hline
        $u=x$&$dv=e^{3x}dx$\\
        \hline
        $du=dx$&$v=\frac{1}{3}e^{3x}$\\
        \hline
    \end{tabular}
\end{table}
\begin{align*}
    \frac{1}{3}x^{2}e^{3x}-\frac{2}{3}\int xe^{3x}dx&=\frac{1}{3}x^{2}e^{3x}-\frac{2}{3}\big(\frac{1}{3}xe^{3x}-\frac{1}{3}\int e^{3x}dx\big)=\frac{1}{3}x^{2}e^{3x}-\frac{2}{3}\big(\frac{1}{3}xe^{3x}-\frac{1}{9}e^{3x}\big)+C\\
    &=\frac{1}{3}e^{3x}(x^{2}-\frac{2}{3}x+\frac{2}{9})+C
\end{align*}
\end{proof}
\begin{problem}
Evaluate $\int_{0}^{4\pi^{2}}\sin(\sqrt{y})dy$
\end{problem}
\begin{proof}[Solution]
Let $x=\sqrt{y}$. Then $dx=\frac{1}{2\sqrt{y}}dy\Rightarrow dy=2\sqrt{y}dx=2xdx$.
\begin{table}[H]
    \centering
    \begin{tabular}{|c|c|}
        \hline
        $u=x$&$dv=2\sin(x)dx$\\
        \hline
        $du=dx$&$v=-2\cos(x)$\\
        \hline
    \end{tabular}
\end{table}
\begin{align*}
    \int\sin(\sqrt{y})dy&=\int x\sin(y)dx=-2x\cos(x)-\int(-2\cos(x))dx=-2x\cos(x)+2\sin(x)\\
    \Rightarrow \int_{0}^{4\pi^{2}}\sin(\sqrt{y})dy&=[-2\sqrt{y}\cos(\sqrt{y})+2\sin(\sqrt{y})]_{0}^{4\pi^{2}}=-4\pi
\end{align*}
\end{proof}
\begin{problem}
Evaluate $\int_{0}^{\ln(\sqrt{3})}\frac{1}{\pi}\frac{e^{t}}{1+e^{2t}}dt$
\end{problem}
\begin{proof}[Solution]
Let $u=e^{t}$. Then $du=e^{t}dt$. So:
\begin{align*}
    \int\frac{1}{\pi}\frac{e^{t}}{1+e^{2t}}dt&=\int\frac{1}{\pi}\frac{1}{1+u^{2}}du=\frac{1}{\pi}\arctan(u)=\frac{1}{\pi}\arctan(e^{t})\\
    \Rightarrow\int_{0}^{\ln(\sqrt{3})}\frac{1}{\pi}\frac{e^{t}}{1+e^{2t}}dt&=\frac{1}{\pi}\arctan(e^{t})\big|_{0}^{\ln(\sqrt{3})}=\frac{1}{\pi}(\arctan(e^{\ln(\sqrt{3})})-\arctan(e^{0}))\\
    &=\frac{1}{\pi}(\arctan(\sqrt{3})-\arctan(1))=\frac{1}{\pi}(\frac{\pi}{\pi}{3}-\frac{\pi}{4})=\frac{1}{12}
\end{align*}
\end{proof}
\newpage
\subsection{Exam II}
\begin{problem}
Evaluate the integral $\int\sin^{5}(x)dx$
\end{problem}
\begin{proof}[Solution]
\begin{equation*}
    \int\sin^{5}(x)dx=\int\sin(x)\sin^{4}(x)dx=\int\sin(x)(1-\cos^{2}(x))^{2}dx
\end{equation*}
Let $u=\cos(x)$. Then $du=-\sin(x)dx$.
\begin{align*}
    \int\sin^{5}(x)dx&=-\int(1-u^{2})^{2}du=-u+\frac{2}{3}u^{3}-\frac{1}{5}u^{5}+C\\
    &=-\cos(x)+\frac{2}{3}\cos^{3}(x)-\frac{1}{5}\cos^{5}(x)+C
\end{align*}
\end{proof}
\begin{problem}
Estimate the integral $\int_{0}^{4}(x^{3}+1)dx$ with $n=4$ using the trapezoidal rule and Simpson's rule.
\end{problem}
\begin{proof}[Solution]
The integral is $f(x)=x^{3}+1$. We have that $\Delta x=\frac{b-a}{n}=\frac{4-0}{4}=1$
\begin{enumerate}
    \item Using the trapazoidal rule:
    \begin{equation*}
        T=\frac{\Delta x}{2}[f(x_{0})+2f(x_{1})+2f(x_{2})+2f(x_{3})+f(x_{4})]=\frac{1}{2}[1+2(2)+2(9)+2(28)+65]=\frac{144}{2}=72
    \end{equation*}
    \item Using Simpson's Rule:
    \begin{equation*}
        T=\frac{\Delta x}{3}[f(x_{0})+4f(x_{1})+2f(x_{2})+4f(x_{3})+f(x_{4})]=\frac{1}{3}[1+4(2)+2(9)+4(28)+65]=\frac{204}{3}=68
    \end{equation*}
\end{enumerate}
\end{proof}
\begin{problem}
Evaluate the integral of $\int\frac{x^{2}}{x^{2}+25}dx$ using trigonometric substitution.
\end{problem}
\begin{proof}[Solution]

\end{proof}
\end{document}