\documentclass[crop=false,class=book,oneside]{standalone}
%----------------------------Preamble-------------------------------%
\input{../../../preamble.tex}
\graphicspath{{../../../images/}}   % Path to Image Folder.
%--------------------------Main Document----------------------------%
\begin{document}
    \ifx\ifmathcourses\undefined
        \title{Chaos Theory}
        \author{Ryan Maguire}
        \date{\vspace{-5ex}}
        \maketitle
        \tableofcontents
        \chapter*{Chaos Theory}
        \markboth{}{CHAOS THEORY}
        \setcounter{chapter}{1}
    \else
        \chapter{Chaos Theory}
    \fi
    \section{Miscellaneous Notes}
        \subsection{Notes from Fall 2016 (UML)}
            \subsubsection{Notes on the Jordan Normal Form}
                Every square matrix $A$ is similar to an upper
                triangular matrix $J$ in
                \textit{Jordan normal form} whose diagonal entries
                are the eigenvalues of $A$. That is, there exists
                an invertible matrix $P$ such that
                $P^{-1}AP=J$. The trace of $A$ is equal to the
                trace of $J$:
                \begin{equation*}
                    \Tr(J)
                    =\Tr(P^{-1}AP)
                    =\Tr(P^{-1}PA)
                    =\Tr(IA)=\Tr(A)
                \end{equation*}
            \subsubsection{Notes on Conjugacy}
                We have:
                \begin{align*}
                    X'(t)&=AX(t),
                    \quad
                    X(0)=X_{0}\\
                    \Rightarrow
                    X(t)&=e^{tA}X_{0}\\
                    \Rightarrow
                    \phi^{A}(t,X_{0})
                    &=e^{tA}X_{0}
                \end{align*}
                Thus, if $B=T^{-1}AT$, for some matrix $T$, then:
                \begin{align*}
                    Y'(t)&=BY(t),
                    \quad
                    Y(0)=Y_{0}\\
                    &=T^{-1}ATY(t)\\
                    \Rightarrow
                    Y(t)
                    &=e^{tT^{-1}AT}Y_{0}\\
                    &=T^{-1}e^{tA}TY_{0}\\
                    \Rightarrow
                    \phi^{B}(t,Y_{0})
                    &=T^{-1}e^{tA}TY_{0}
                \end{align*}
                Thus, the homeomorphism is $h(X)=T^{-1}X$,
                and we have:
                \begin{equation*}
                    \phi^{B}(t,h(X_{0}))
                    =\phi^{B}(t,T^{-1}X_{0})
                    =T^{-1}e^{tA}T(T^{-1}X_{0})
                    =T^{-1}e^{tA}X_{0}
                    =h(\phi^{A}(t,X_{0}))
                \end{equation*}
\end{document}